proofs/AllocFree.fst
@@ -14,7 +14,8 @@ let post_alloc (s : state) : prop =
     s._3 == Ok /\ 
     s._1 "x" == Loc l /\ 
     l =!= 0 /\ 
-    points_to l v s
+    points_to l v s /\
+    (exists x_old. emp (override s._1 "x" x_old, override s._2 l Empty, Ok))
 
 let pre_free (s:state) : prop = 
   s._3 == Ok /\ post_alloc s
@@ -33,16 +34,19 @@ let post_uaf_err (s : state) : prop =
   points_to_empty (eval_expr s (Var "x")) s /\
   pre_store (s._1, s._2, Ok)
 
-let prog_uaf=
+let prog_uaf =
   (Alloc "x") `Seq`
   ((Free (Var "x")) `Seq`
   (Store (Var "x") (Const 1)))
 
 let proof_uaf : isl_triple emp prog_uaf post_uaf_err =
-  let p_alloc = ISL_Alloc1 "x" in
-  let p_free = ISL_Free (Var "x") in
-  let p_store = ISL_StoreEr (Var "x") (Const 1) in
+  let p_alloc = ISL_Alloc1 #emp "x" in
+  let p_free_raw = ISL_Free #pre_free (Var "x") in
+  let p_store = ISL_StoreEr #pre_store (Var "x") (Const 1) in
+
+  let p_free = ISL_Consequence pre_free post_free p_free_raw () () in
 
   let p_seq1 = ISL_Seq p_free p_store in
   let p_seq2 = ISL_Seq p_alloc p_seq1 in
+  
   ISL_Consequence emp post_uaf_err p_seq2 () ()
